Exception data propogated from L2 and L3 to L4 for better failure info.  Olivier's bug NOT fixed yet.  (I'm working on a partial fix, but a good fix requires work on template-coq.)

theories/L2_typeStrippedL1/test_wcbvEval.v
@@ -19,6 +19,16 @@ Definition exc_wcbvEval (tmr:nat) (pgm:program): option Term :=
     | Some pgm => wcbvEval tmr (L2.program.env pgm) (L2.program.main pgm)
   end.
 
+(** Olivier's example **)
+Definition olivier := (Some 0).
+Quote Recursively Definition p_olivier := olivier.
+Quote Definition q_olivier := Eval cbv in olivier.
+Print p_olivier.
+Print q_olivier.
+Goal (exc_wcbvEval 10 p_olivier) = term_Term q_olivier.
+compute. reflexivity.
+Qed.
+
 Inductive foo (A:Set) : Set :=
 | nilf: foo A
 | consf: (fun (Y W:Set) => Y -> foo Y -> foo ((fun X Z => X) A nat)) A bool.
